Instantiated new loc with locations+permissions

ulib/FStar.MG2.fst
@@ -192,49 +192,60 @@ type ucell : Type0 = {
   b_pid:perm_id;
 }
 
-let ucell_preserved (b:ucell) (h0 h1:HS.mem) : GTot Type0 =
-  forall (t:Type0) (b':array t).
-    (let i = b.b_index - U32.v b'.idx in // This cell corresponds to index i in the buffer
-      (frameOf b' == b.b_rid /\ as_addr b' == b.b_addr /\ b'.pid == (Ghost.hide b.b_pid) /\ U32.v b'.max_length == b.b_max /\
-        b.b_index >= U32.v b'.idx /\ b.b_index < U32.v b'.idx + U32.v b'.length /\ // If this cell is part of the buffer
-        live_cell h0 b' i ==>
-          live_cell h1 b' i /\ // If this cell is preserved, then its liveness is preserved
-          (sel h0 b' i == sel h1 b' i))) // And its contents (snapshot + permission) are the same
+let ucell_matches_array_cell (cell: ucell) (t:Type) (b: array t) (h: HS.mem) =
+frameOf b = cell.b_rid /\ as_addr b = cell.b_addr /\ U32.v b.max_length = cell.b_max /\ HS.contains h b.content /\
+     cell.b_index >= U32.v b.idx /\ cell.b_index < U32.v b.idx + U32.v b.length // If this cell is part of the buffer
 
-let prove_loc_preserved (loc: ucell) (h0 h1: HS.mem)
+let ucell_matches_used_array_cell (cell: ucell) (t:Type) (b: array t) (h: HS.mem) =
+  ucell_matches_array_cell cell t b h /\ begin
+    let (_, perm_map) = Seq.index (HS.sel h b.content) cell.b_index in
+    cell.b_pid <= get_current_max (Ghost.reveal perm_map)
+  end
+
+let ucell_matches_unused_array_cell (cell: ucell) (t:Type) (b: array t) (h: HS.mem) =
+  ucell_matches_array_cell cell t b h /\ begin
+    let (_, perm_map) = Seq.index (HS.sel h b.content) cell.b_index in
+    cell.b_pid > get_current_max (Ghost.reveal perm_map)
+  end
+
+let ucell_matches_live_array_cell (cell: ucell) (t:Type) (b: array t) (h: HS.mem) =
+  ucell_matches_used_array_cell cell t b h /\ begin
+    let i = cell.b_index - U32.v b.idx in
+    live_cell h b i
+  end
+
+let ucell_preserved (cell:ucell) (h0 h1:HS.mem) : GTot Type0 =
+  forall (t:Type0) (b':array t). begin let i = cell.b_index - U32.v b'.idx in // This cell corresponds to index i in the buffer
+    ucell_matches_live_array_cell cell t b' h0 ==>
+      (ucell_matches_live_array_cell cell t b' h1 /\  // If this cell is preserved, then its liveness is preserved
+      sel h0 b' i == sel h1 b' i) // And its contents (snapshot + permission) are the same
+  end
+
+let ucell_preserved_intro (loc: ucell) (h0 h1: HS.mem)
   (lemma: (t: Type0 -> b': array t -> Lemma
     (requires (
       let i = loc.b_index - U32.v b'.idx in
-      frameOf b' == loc.b_rid /\ as_addr b' == loc.b_addr /\
-      Ghost.reveal b'.pid == loc.b_pid /\ U32.v b'.max_length == loc.b_max /\
-      loc.b_index >= U32.v b'.idx /\ loc.b_index < U32.v b'.idx + U32.v b'.length /\
-      live_cell h0 b' i))
+      ucell_matches_live_array_cell loc t b' h0))
     (ensures (
       let i = loc.b_index - U32.v b'.idx in
-      live_cell h1 b' i /\
+      ucell_matches_live_array_cell loc t b' h1 /\
       sel h0 b' i  == sel h1 b' i
       ))
   )) : Lemma (ucell_preserved loc h0 h1)
   =
   let aux (t: Type0) (b':array t) : Lemma(
       let i = loc.b_index - U32.v b'.idx in
-      frameOf b' == loc.b_rid /\ as_addr b' == loc.b_addr /\
-      Ghost.reveal b'.pid == loc.b_pid /\ U32.v b'.max_length == loc.b_max /\
-      loc.b_index >= U32.v b'.idx /\ loc.b_index < U32.v b'.idx + U32.v b'.length /\
-      live_cell h0 b' i ==>
-        live_cell h1 b' i /\
-        sel h0 b' i  == sel h1 b' i)
+      ucell_matches_live_array_cell loc t b' h0 ==>
+      ucell_matches_live_array_cell loc t b' h1 /\
+      sel h0 b' i  == sel h1 b' i)
   =
   let aux' (_ : squash (
       let i = loc.b_index - U32.v b'.idx in
-      frameOf b' == loc.b_rid /\ as_addr b' == loc.b_addr /\
-      Ghost.reveal b'.pid == loc.b_pid /\ U32.v b'.max_length == loc.b_max /\
-      loc.b_index >= U32.v b'.idx /\ loc.b_index < U32.v b'.idx + U32.v b'.length /\
-      live_cell h0 b' i)
+      ucell_matches_live_array_cell loc t b' h0)
     ) : Lemma (
       let i = loc.b_index - U32.v b'.idx in
       loc.b_index >= U32.v b'.idx /\ loc.b_index < U32.v b'.idx + U32.v b'.length /\
-      live_cell h1 b' i /\
+      ucell_matches_live_array_cell loc t b' h1 /\
       sel h0 b' i  == sel h1 b' i
     )
     = lemma t b'
@@ -256,35 +267,45 @@ let ucell_includes (c1 c2: ucell) : GTot Type0 =
 let ucell_disjoint (c1 c2:ucell) : GTot Type0 =
   (c1.b_rid <> c2.b_rid) \/
   (c1.b_addr <> c2.b_addr) \/
-  (c1.b_max == c2.b_max /\
+  ((c1.b_max = c2.b_max) /\ // At this point c1 and c2 point to the same allocated array
     (c1.b_index <> c2.b_index \/           // Either the cells are different (i.e. spatially disjoint)
     c1.b_pid <> c2.b_pid))                 // Or they don't have the same permission
 
-let live_ucell_matches_array (cell: ucell) (t:Type) (b: array t) (h: HS.mem) =
-frameOf b = cell.b_rid /\ as_addr b = cell.b_addr /\ U32.v b.max_length = cell.b_max /\ HS.contains h b.content /\
-     cell.b_index >= U32.v b.idx /\ cell.b_index < U32.v b.idx + U32.v b.length /\ // If this cell is part of the buffer
-     live_cell h b (cell.b_index - U32.v b.idx)
-
 let ucell_unused_in (cell:ucell) (h: HS.mem) =
-  forall (t:Type) (b:array t).
-    live_ucell_matches_array cell t b h ==>
-    begin
-      let (_, perm_map) = Seq.index (HS.sel h b.content) cell.b_index in
-      cell.b_pid > get_current_max (Ghost.reveal perm_map)
-    end
-
-
+  // Either there is nothing allocated at that memory cell
+  (forall (t:Type) (ref: HS.mreference t (Heap.trivial_preorder t)).
+    (HS.as_addr ref = cell.b_addr /\ HS.frameOf ref = cell.b_rid) ==> (~ (HS.contains h ref))
+  ) \/
+  // Or there is an allocated array but it doesnt use the ucell
+  (exists (t:Type) (b:array t). ucell_matches_unused_array_cell cell t b h)
 
 let ucell_used_in (cell:ucell) (h: HS.mem) =
-  let used_in  (t:Type) (b:array t) =
-    live_ucell_matches_array cell t b h ==>
-    begin
-      let (_, perm_map) = Seq.index (HS.sel h b.content) cell.b_index in
-      cell.b_pid <= get_current_max (Ghost.reveal perm_map)
-    end
-  in
-  (forall (t:Type) (b:array t). used_in t b) /\
-  (exists (t:Type) (b:array t). used_in t b)
+  // There exists an array allocated with the correct size that contains a live cell corresponding to the ucell
+  exists (t:Type) (b:array t). ucell_matches_live_array_cell cell t b h
+
+
+let live_same_arrays_equal_types
+  (#a1: Type0)
+  (#a2: Type0)
+  (b1: array a1{U32.v b1.max_length > 0})
+  (b2: array a2{U32.v b2.max_length > 0})
+  (h: HS.mem)
+  : Lemma (requires (
+     frameOf b1 == frameOf b2 /\
+     as_addr b1 == as_addr b2 /\
+     HS.contains h b1.content /\
+     HS.contains h b2.content))
+   (ensures (a1 == a2 /\ HS.sel h b1.content == HS.sel h b2.content /\ b1.max_length = b2.max_length))
+  =
+  Heap.lemma_distinct_addrs_distinct_preorders ();
+  Heap.lemma_distinct_addrs_distinct_mm ();
+  let s1 = HS.sel h b1.content in
+  let s2 = HS.sel h b2.content in
+  let (_, vp1) = Seq.index s1 0 in
+  let (_, vp2) = Seq.index s2 0 in
+  Seq.lemma_equal_instances_implies_equal_types ()
+
+#set-options "--z3rlimit 30"
 
 let cls_ucell : cls ucell = Cls #ucell
   ucell_includes
@@ -299,19 +320,85 @@ let cls_ucell : cls ucell = Cls #ucell
   (fun x h1 h2 h3 -> ())
   ucell_used_in
   ucell_unused_in
-  (fun x y h ->
+  (fun x1 x2 h ->
     (* used_in and unused_in disjoint *)
-    let aux (_ : squash(x `ucell_used_in` h /\ y `ucell_unused_in` h)) : Lemma
-      (x `ucell_disjoint` y)
-      = admit()
+    let aux (_ : squash(x1 `ucell_used_in` h /\ x2 `ucell_unused_in` h)) : Lemma
+      (x1 `ucell_disjoint` x2)
+      =
+      let p (t: Type) = exists (b: array t). ucell_matches_live_array_cell x1 t b h in
+      let pf : squash (exists (t: Type) . p t) = () in
+      Classical.exists_elim (x1 `ucell_disjoint` x2) #Type #p pf (fun t ->
+        let p (b: array t) = ucell_matches_live_array_cell x1 t b h in
+        let pf : squash (exists (b: array t) . p b) = () in
+        Classical.exists_elim (x1 `ucell_disjoint` x2) #(array t) #p pf (fun b ->
+          let case1 = forall (t':Type) (ref: HS.mreference t' (Heap.trivial_preorder t')).
+           (HS.as_addr ref = x2.b_addr /\ HS.frameOf ref = x2.b_rid) ==> (~ (HS.contains h ref))
+          in
+          let case2 = (exists (t':Type) (b':array t'). ucell_matches_unused_array_cell x2 t' b' h) in
+          Classical.or_elim
+            #case1 #case2 #(fun _ -> x1 `ucell_disjoint` x2)
+            (fun (_ : squash (case1)) ->
+              if (x1.b_rid <> x2.b_rid || x1.b_addr <> x2.b_addr) then () else
+                assert((HS.contains h b.content) /\ ~ (HS.contains h b.content))
+            )
+            (fun (_ : squash (case2)) ->
+              let p (t': Type) = exists (b': array t'). ucell_matches_unused_array_cell x2 t' b' h in
+              let pf : squash (exists (t': Type) . p t') = () in
+              Classical.exists_elim (x1 `ucell_disjoint` x2) #Type #p pf (fun t' ->
+                let p (b': array t') = ucell_matches_unused_array_cell x2 t' b' h in
+                let pf : squash (exists (b': array t') . p b') = () in
+                Classical.exists_elim (x1 `ucell_disjoint` x2) #(array t') #p pf (fun b' ->
+                  if (x1.b_rid <> x2.b_rid || x1.b_addr <> x2.b_addr) then () else begin
+                    live_same_arrays_equal_types b' b h;
+                    if x1.b_index <> x2.b_index then () else begin
+                      let (_, perm_map1) = Seq.index (HS.sel h b.content) x1.b_index in
+                      let (_, perm_map2) = Seq.index (HS.sel h b'.content) x2.b_index in
+                      if x1.b_pid <> x2.b_pid then () else begin
+                        assert(perm_map1 == perm_map2);
+                        assert(
+                          x1.b_pid <= get_current_max (Ghost.reveal perm_map1) /\
+                          x1.b_pid > get_current_max (Ghost.reveal perm_map1)
+                        )
+                      end
+                    end
+                  end
+                )
+              )
+            )
+        )
+      )
     in
     Classical.impl_intro aux
   )
   (fun greater lesser h -> ())
   (fun greater lesser h -> ())
-  (fun x h1 h2 ->
-    (* aloc_unused_in_preserved *)
-    admit()
+  (fun x h0 h1 ->
+    ucell_preserved_intro x h0 h1 (fun t b ->
+      let i = x.b_index - U32.v b.idx in
+      let case1 = forall (t':Type) (ref: HS.mreference t' (Heap.trivial_preorder t')).
+        (HS.as_addr ref = x.b_addr /\ HS.frameOf ref = x.b_rid) ==> (~ (HS.contains h0 ref))
+      in
+      let case2 = exists (t':Type) (b':array t').
+        ucell_matches_unused_array_cell x t' b' h0
+      in
+      let goal = ucell_matches_live_array_cell x t b h1 /\ sel h0 b i  == sel h1 b i in
+      Classical.or_elim #case1 #case2 #(fun _ -> goal)
+        (fun (_ : squash (case1)) -> assert((HS.contains h1 b.content) /\ (~ (HS.contains h1 b.content))))
+        (fun (_ : squash (case2)) ->
+          let p (t': Type) = exists (b': array t'). ucell_matches_unused_array_cell x t' b' h0 in
+          let pf : squash (exists (t': Type) . p t') = () in
+          Classical.exists_elim goal #Type #p pf (fun t' ->
+            let p (b': array t') = ucell_matches_unused_array_cell x t' b' h0 in
+            let pf : squash (exists (b': array t') . p b') = () in
+            Classical.exists_elim goal #(array t') #p pf (fun b' ->
+              live_same_arrays_equal_types b' b h0;
+              let (_, perm_map) = Seq.index (HS.sel h0 b.content) x.b_index in
+              LowStar.Permissions.lemma_greater_max_not_live_pid (Ghost.reveal perm_map) x.b_pid;
+              assert((live_cell h0 b i) /\ (~ (live_cell h0 b i)))
+            )
+          )
+        )
+    )
   )
 
 let loc_ucell = loc cls_ucell
